n_mutualExAbs1_base1.thy
@@ -1,0 +1,905 @@
+(*  Title:      HOL/Auth/n_mutualExAbs1_base.thy
+    Author:     Yongjian Li and Kaiqiang Duan, State Key Lab of Computer Science, Institute of Software, Chinese Academy of Sciences
+    Copyright    2016 State Key Lab of Computer Science, Institute of Software, Chinese Academy of Sciences
+*)
+ 
+theory n_mutualExAbs1_base1 imports paraTheory
+begin
+
+section{*Main definitions*}
+
+subsection{* Definitions of Constants*}
+definition I::"scalrValueType" where [simp]: "I\<equiv> enum ''control'' ''I''"
+definition T::"scalrValueType" where [simp]: "T\<equiv> enum ''control'' ''T''"
+definition C::"scalrValueType" where [simp]: "C\<equiv> enum ''control'' ''C''"
+definition E::"scalrValueType" where [simp]: "E\<equiv> enum ''control'' ''E''"
+definition true::"scalrValueType" where [simp]: "true\<equiv> boolV True"
+definition false::"scalrValueType" where [simp]: "false\<equiv> boolV False"
+
+
+
+subsection{*  Definitions of Parameterized Rules *}
+
+definition n_Try::"nat \<Rightarrow> rule" where [simp]:
+"n_Try  i\<equiv>
+let g = (eqn (IVar (Field (Para (Ident ''n'') i) ''st'')) (Const I)) in
+let s = (parallelList [(assign ((Field (Para (Ident ''n'') i) ''st''), (Const T)))]) in
+guard g s"
+
+definition n_Crit::"nat \<Rightarrow> rule" where [simp]:
+"n_Crit  i\<equiv>
+let g = (andForm (eqn (IVar (Field (Para (Ident ''n'') i) ''st'')) (Const T)) (eqn (IVar (Ident ''x'')) (Const true))) in
+let s = (parallelList [(assign ((Field (Para (Ident ''n'') i) ''st''), (Const C))), (assign ((Ident ''x''), (Const false))), (assign ((Field (Para (Ident ''n'') i) ''data''), (IVar (Ident ''memDATA''))))]) in
+guard g s"
+
+definition n_Exit::"nat \<Rightarrow> rule" where [simp]:
+"n_Exit  i\<equiv>
+let g = (eqn (IVar (Field (Para (Ident ''n'') i) ''st'')) (Const C)) in
+let s = (parallelList [(assign ((Field (Para (Ident ''n'') i) ''st''), (Const E)))]) in
+guard g s"
+
+definition n_Idle::"nat \<Rightarrow> rule" where [simp]:
+"n_Idle  i\<equiv>
+let g = (eqn (IVar (Field (Para (Ident ''n'') i) ''st'')) (Const E)) in
+let s = (parallelList [(assign ((Field (Para (Ident ''n'') i) ''st''), (Const I))), (assign ((Ident ''x''), (Const true))), (assign ((Ident ''memDATA''), (IVar (Field (Para (Ident ''n'') i) ''data''))))]) in
+guard g s"
+
+definition n_Store::"nat \<Rightarrow> nat \<Rightarrow> rule" where [simp]:
+"n_Store  i data\<equiv>
+let g = (eqn (IVar (Field (Para (Ident ''n'') i) ''st'')) (Const C)) in
+let s = (parallelList [(assign ((Field (Para (Ident ''n'') i) ''st''), (Const C))), (assign ((Ident ''x''), (Const false))), (assign ((Ident ''auxDATA''), (Const (index data)))), (assign ((Field (Para (Ident ''n'') i) ''data''), (Const (index data))))]) in
+guard g s"
+
+definition n_ABS_Store::"nat \<Rightarrow> nat \<Rightarrow> rule" where [simp]:
+"n_ABS_Store N data\<equiv>
+let g = (forallForm (down N) (\<lambda>j. (andForm (neg (eqn (IVar (Field (Para (Ident ''n'') j) ''st'')) (Const C))) (neg (eqn (IVar (Field (Para (Ident ''n'') j) ''st'')) (Const E)))))) in
+let s = (parallelList [(assign ((Ident ''x''), (Const false))), (assign ((Ident ''auxDATA''), (Const (index data))))]) in
+guard g s"
+
+definition n_ABS_Crit::"rule" where [simp]:
+"n_ABS_Crit  \<equiv>
+let g = (eqn (IVar (Ident ''x'')) (Const true)) in
+let s = (parallelList [(assign ((Ident ''x''), (Const false)))]) in
+guard g s"
+
+definition n_ABS_Idle::"nat \<Rightarrow> rule" where [simp]:
+"n_ABS_Idle N \<equiv>
+let g = (forallForm (down N) (\<lambda>j. (andForm (neg (eqn (IVar (Field (Para (Ident ''n'') j) ''st'')) (Const C))) (neg (eqn (IVar (Field (Para (Ident ''n'') j) ''st'')) (Const E)))))) in
+let s = (parallelList [(assign ((Ident ''x''), (Const true))), (assign ((Ident ''memDATA''), (IVar (Ident ''auxDATA''))))]) in
+guard g s"
+
+
+
+
+
+subsection{*The set of All actual Rules w.r.t. a Protocol Instance with Size $N$*}
+definition rules::"nat \<Rightarrow> rule set" where [simp]:
+"rules N \<equiv> {r.
+(\<exists> i. i\<le>N\<and>r=n_Try  i) \<or>
+(\<exists> i. i\<le>N\<and>r=n_Crit  i) \<or>
+(\<exists> i. i\<le>N\<and>r=n_Exit  i) \<or>
+(\<exists> i. i\<le>N\<and>r=n_Idle  i)
+}"
+
+definition  NC::"nat " where [simp]: "NC==1" 
+
+definition rulesAbs::"nat \<Rightarrow> rule set" where [simp]:
+"rulesAbs  N\<equiv> {r.
+(\<exists> i. i\<le>NC\<and>r=n_Crit  i) \<or>
+(\<exists> i. i\<le>NC\<and>r=n_Exit  i) \<or>
+(\<exists> i. i\<le>NC\<and>r=n_Idle  i) \<or>
+(\<exists> i. i\<le>NC\<and>r=n_Try  i) \<or>
+(\<exists> i data. i\<le>NC\<and>data\<le>N\<and>r=n_Store  i data) \<or>
+(\<exists> data. data\<le>N\<and>r=n_ABS_Store NC data) \<or>
+(r=n_ABS_Crit  ) \<or>
+(r=n_ABS_Idle NC )
+}"
+
+
+
+subsection{*Definitions of a Formally Parameterized Invariant Formulas*}
+
+
+
+subsection{*Definitions of  the Set of Invariant Formula Instances in a $N$-protocol Instance*}
+definition inv__1::"nat \<Rightarrow> nat \<Rightarrow> formula" where [simp]:
+"inv__1 p__Inv0 p__Inv1 \<equiv>
+(neg (andForm (eqn (IVar (Field (Para (Ident ''n'') p__Inv0) ''st'')) (Const C)) (eqn (IVar (Field (Para (Ident ''n'') p__Inv1) ''st'')) (Const C))))"
+
+definition inv__2::"nat \<Rightarrow> formula" where [simp]:
+"inv__2 p__Inv0 \<equiv>
+(neg (andForm (eqn (IVar (Field (Para (Ident ''n'') p__Inv0) ''st'')) (Const C)) (neg (eqn (IVar (Field (Para (Ident ''n'') p__Inv0) ''data'')) (IVar (Ident ''auxDATA''))))))"
+
+definition inv__3::"nat \<Rightarrow> formula" where [simp]:
+"inv__3 p__Inv0 \<equiv>
+(neg (andForm (eqn (IVar (Field (Para (Ident ''n'') p__Inv0) ''st'')) (Const E)) (neg (eqn (IVar (Field (Para (Ident ''n'') p__Inv0) ''data'')) (IVar (Ident ''auxDATA''))))))"
+
+definition inv__4::"nat \<Rightarrow> nat \<Rightarrow> formula" where [simp]:
+"inv__4 p__Inv0 p__Inv1 \<equiv>
+(neg (andForm (eqn (IVar (Field (Para (Ident ''n'') p__Inv0) ''st'')) (Const C)) (eqn (IVar (Field (Para (Ident ''n'') p__Inv1) ''st'')) (Const E))))"
+
+definition inv__5::"nat \<Rightarrow> nat \<Rightarrow> formula" where [simp]:
+"inv__5 p__Inv0 p__Inv1 \<equiv>
+(neg (andForm (eqn (IVar (Field (Para (Ident ''n'') p__Inv0) ''st'')) (Const E)) (eqn (IVar (Field (Para (Ident ''n'') p__Inv1) ''st'')) (Const E))))"
+
+definition inv__6::"nat \<Rightarrow> nat \<Rightarrow> formula" where [simp]:
+"inv__6 p__Inv0 p__Inv1 \<equiv>
+(neg (andForm (eqn (IVar (Field (Para (Ident ''n'') p__Inv0) ''st'')) (Const E)) (eqn (IVar (Field (Para (Ident ''n'') p__Inv1) ''st'')) (Const C))))"
+
+definition inv__7::"formula" where [simp]:
+"inv__7  \<equiv>
+(neg (andForm (eqn (IVar (Ident ''x'')) (Const true)) (neg (eqn (IVar (Ident ''memDATA'')) (IVar (Ident ''auxDATA''))))))"
+
+definition inv__8::"nat \<Rightarrow> formula" where [simp]:
+"inv__8 p__Inv0 \<equiv>
+(neg (andForm (eqn (IVar (Field (Para (Ident ''n'') p__Inv0) ''st'')) (Const C)) (eqn (IVar (Ident ''x'')) (Const true))))"
+
+definition inv__9::"nat \<Rightarrow> formula" where [simp]:
+"inv__9 p__Inv0 \<equiv>
+(neg (andForm (eqn (IVar (Field (Para (Ident ''n'') p__Inv0) ''st'')) (Const E)) (eqn (IVar (Ident ''x'')) (Const true))))"
+
+subsection{*Definitions of  the Set of Invariant Formula Instances in a $N$-protocol Instance*}
+definition invariants::"nat \<Rightarrow> formula set" where [simp]:
+"invariants N \<equiv> {f.
+(\<exists> p__Inv0 p__Inv1. p__Inv0\<le>N\<and>p__Inv1\<le>N\<and>p__Inv0~=p__Inv1\<and>f=inv__1  p__Inv0 p__Inv1) \<or>
+(\<exists> p__Inv0. p__Inv0\<le>N\<and>f=inv__2  p__Inv0) \<or>
+(\<exists> p__Inv0. p__Inv0\<le>N\<and>f=inv__3  p__Inv0) \<or>
+(\<exists> p__Inv0 p__Inv1. p__Inv0\<le>N\<and>p__Inv1\<le>N\<and>p__Inv0~=p__Inv1\<and>f=inv__4  p__Inv0 p__Inv1) \<or>
+(\<exists> p__Inv0 p__Inv1. p__Inv0\<le>N\<and>p__Inv1\<le>N\<and>p__Inv0~=p__Inv1\<and>f=inv__5  p__Inv0 p__Inv1) \<or>
+(\<exists> p__Inv0 p__Inv1. p__Inv0\<le>N\<and>p__Inv1\<le>N\<and>p__Inv0~=p__Inv1\<and>f=inv__6  p__Inv0 p__Inv1) \<or>
+(f=inv__7  ) \<or>
+(\<exists> p__Inv0. p__Inv0\<le>N\<and>f=inv__8  p__Inv0) \<or>
+(\<exists> p__Inv0. p__Inv0\<le>N\<and>f=inv__9  p__Inv0)
+}"
+
+definition invariantsAbs::" formula list" where [simp]:
+"invariantsAbs  \<equiv> 
+
+[
+(inv__1  0 1) ,(inv__1   1 0),
+(inv__2  0),(inv__2  1),
+(inv__3 0),(inv__3 1),
+(inv__4  0 1),(inv__4   1 0),
+(inv__5  0 1),(inv__5   1 0),
+(inv__6  0 1) ,(inv__6   1 0),
+(inv__7  ) ,
+(inv__8  0) ,(inv__8  1),
+(inv__9  0),(inv__9  1)
+]"
+(*[
+(inv__1  0 1),  
+(inv__2  0), 
+(inv__3 0), 
+(inv__4  0 1), 
+(inv__5  0 1), 
+(inv__6  0 1) , 
+(inv__7  ) ,
+(inv__8  0) , 
+(inv__9  0)
+]"*)
+
+
+subsection{*Definitions of initial states*}
+
+definition initSpec0::"nat \<Rightarrow> formula" where [simp]:
+"initSpec0 N \<equiv> (forallForm (down N) (% i . (eqn (IVar (Field (Para (Ident ''n'') i) ''st'')) (Const I))))"
+
+definition initSpec1::"nat \<Rightarrow> formula" where [simp]:
+"initSpec1 N \<equiv> (forallForm (down N) (% i . (eqn (IVar (Field (Para (Ident ''n'') i) ''data'')) (Const (index 1)))))"
+
+definition initSpec2::"formula" where [simp]:
+"initSpec2  \<equiv> (eqn (IVar (Ident ''x'')) (Const true))"
+
+definition initSpec3::"formula" where [simp]:
+"initSpec3  \<equiv> (eqn (IVar (Ident ''auxDATA'')) (Const (index 1)))"
+
+definition initSpec4::"formula" where [simp]:
+"initSpec4  \<equiv> (eqn (IVar (Ident ''memDATA'')) (Const (index 1)))"
+
+definition allInitSpecs::"nat \<Rightarrow> formula list" where [simp]:
+"allInitSpecs N \<equiv> [
+(initSpec0 N),
+(initSpec1 N),
+(initSpec2 ),
+(initSpec3 ),
+(initSpec4 )
+]"
+
+definition allInitSpecsAbs::" formula list" where [simp]:
+"allInitSpecsAbs  \<equiv> [
+(initSpec0 NC), 
+(initSpec1 NC),
+(initSpec2  ),
+(initSpec3 ),
+(initSpec4 )
+]"
+
+lemma andListMono2Aux: 
+  assumes a1:"formEval a1 s \<longrightarrow> formEval b1 s" and a2:"formEval (andList A) s \<longrightarrow>formEval (andList B) s"
+  shows "formEval (andList (a1#A)) s \<longrightarrow> formEval (andList (b1#B)) s"
+  by (simp add: a2 local.a1)
+  
+lemma andListMono2[intro]: 
+  assumes a1:"formEval a1 s \<longrightarrow> formEval b1 s" and a2:"formEval (andList A) s \<longrightarrow>formEval (andList B) s"
+  and a3:"formEval (andList (a1#A)) s "
+  shows " formEval (andList (b1#B)) s"
+  using a2 a3 local.a1 by auto 
+  
+axiomatization  where axiomOnf2 [simp,intro]:
+   "s \<in> reachableSet (set (allInitSpecs N )) (rules N) \<Longrightarrow>  1 < N \<Longrightarrow> 1 < i \<Longrightarrow> j<2 \<Longrightarrow>  formEval (f 0 1) s \<Longrightarrow> formEval (f i j) s"
+
+axiomatization  where axiomOnf1 [simp,intro]:
+   "s \<in> reachableSet (set (allInitSpecs N )) (rules N) \<Longrightarrow> 1 < N \<Longrightarrow> 1 < i \<Longrightarrow>formEval (f 0 ) s \<Longrightarrow> formEval (f i) s"
+
+
+ (* apply(simp)
+  apply(erule disjE)
+  apply(rule_tac x="inv__1 0 1" in exI,simp)
+  apply(erule disjE)
+  apply(rule_tac x="inv__1 0 1" in exI,simp)
+  apply(rule_tac x="inv__9 0 " in exI,simp)
+  done*)
+
+lemma lemmaOnIdleLeNc:
+  assumes a1:"i\<le>NC" 
+  shows "trans_sim_on1 (n_Idle  i) (n_Idle  i) (set invariantsAbs) s" (is "trans_sim_on1 ?r ?r ?F s")
+proof(rule ruleSimId)
+  show  "\<forall>v. v\<in>varOfForm (pre ?r) \<longrightarrow>  v \<in>(varOfFormList invariantsAbs) "
+    by(cut_tac a1, auto) 
+    
+next
+  show  b1: "\<forall>v a. a \<in> set (statement2Assigns (act ?r)) \<longrightarrow> v\<in>varOfExp ( substExpByStatement (IVar (fst a))  (act ?r))\<longrightarrow>v \<in>varOfFormList invariantsAbs "
+   proof(cut_tac a1,(rule allI)+,(rule impI)+,auto) qed
+    
+ qed
+
+lemma lemmaOnIdleGtNc1:
+  assumes a1:"i>NC" and a2:"s \<in> reachableSet (set (allInitSpecs N)) (rules N)" and a3:"NC<N" and  
+  a4:"\<forall>f.  f \<in>(set invariantsAbs) \<longrightarrow>  formEval f s"
+  shows "trans_sim_on1 (n_Idle  i) (n_ABS_Idle  NC) (set invariantsAbs) s" (is "trans_sim_on1 ?r ?r' (set ?F) s")
+proof(rule ruleSimCond1)
+  show " formEval (pre ?r) s \<longrightarrow>formEval (pre ?r') s" (is "?A \<longrightarrow>?B")
+  proof(rule impI)+
+    assume b1:"?A"  
+      
+    from a4  have b4:"formEval (inv__5 0 1 ) s"   by (force simp del:inv__5_def)
+    have b5:"formEval (inv__5 i 0 ) s" 
+    proof(cut_tac a1 a2 a3 b4,rule axiomOnf2,force+)qed
+    with b1  have b6:"formEval (neg (eqn (IVar (Field (Para (Ident ''n'') 0) ''st'')) (Const E))) s" by auto
+     have b7:"formEval (inv__5 i 1 ) s" 
+     proof(cut_tac a1 a2 a3 b4,rule axiomOnf2,force+)qed
+     with b1 have b7:"formEval (neg (eqn (IVar (Field (Para (Ident ''n'') 1) ''st'')) (Const E))) s" by auto
+
+      
+     from a4 have b8:"formEval (inv__6 0 1 ) s"    by (force simp del:inv__6_def)
+
+     have b9:"formEval (inv__6 i 0 ) s" 
+    proof(cut_tac a1 a2 a3 b8,rule axiomOnf2,force+)qed
+    with b1 have b9:"formEval (neg (eqn (IVar (Field (Para (Ident ''n'') 0) ''st'')) (Const C))) s" by auto
+     have b10:"formEval (inv__6 i 1 ) s" 
+     proof(cut_tac a1 a2 a3 b8,rule axiomOnf2,force+)qed
+     with b1 have b11:"formEval (neg (eqn (IVar (Field (Para (Ident ''n'') 1) ''st'')) (Const C))) s" by auto
+    
+     from b1 b6 b7 b9 b11 show "formEval (pre ?r') s" 
+       by auto
+   qed
+ next     
+   show "(\<forall>  v. v \<in>  varOfSent (act  ?r') \<longrightarrow>  v \<in> varOfFormList ?F \<longrightarrow> formEval (pre ?r) s \<longrightarrow> 
+    expEval (substExpByStatement (IVar v)  (act ?r')) s = expEval (substExpByStatement (IVar v)  (act ?r)) s)"
+   proof(rule allI,(rule impI)+)
+      fix  v
+     assume b1:"v\<in> (varOfFormList invariantsAbs)"  and b2:"formEval (pre ?r) s" and b4:"v \<in>varOfSent (act ?r')"
+
+     have "(inv__3 0  )\<in>(set invariantsAbs)" by force
+     with a4 have b30:"formEval (inv__3 0 ) s"   apply(drule_tac x="(inv__3 0  )" in spec,blast)done
+
+     have b3:"formEval (inv__3 i ) s"  proof(cut_tac a1 a2 a3 b30,rule axiomOnf1,force+)qed
+
+     show "expEval (substExpByStatement (IVar v)  (act ?r')) s = expEval (substExpByStatement (IVar v)  (act ?r)) s"  
+       apply (cut_tac  a1 b1 b2 b3,auto) done
+   qed
+ next
+   show "\<forall>  v. v \<in>  varOfSent (act ?r) \<longrightarrow>  v \<in> varOfFormList ?F \<longrightarrow> v \<in>  varOfSent (act ?r')" by(cut_tac a1, auto)
+
+  (* have "\<forall>f v va. v \<in> varOfForm f \<longrightarrow> f \<in>?F \<longrightarrow>va\<in>varOfExp ( substExpByStatement (IVar v)  (act ?r'))\<longrightarrow> va \<in>(varOfFormList invariantsAbs)"   by auto
+  a41:" \<forall>  v. v \<in>  varOfSent (act r1) \<longrightarrow>  v \<in> varOfFormList F \<longrightarrow> v \<in>  varOfSent (act r2)" and
+
+  a5:"\<forall> v va. v \<in> varOfSent (act r2) \<longrightarrow>va\<in>varOfExp ( substExpByStatement (IVar v)  (act r2))\<longrightarrow> va \<in> (varOfFormList F *)
+ next show "\<forall> v va. v \<in> varOfSent (act ?r') \<longrightarrow>va\<in>varOfExp ( substExpByStatement (IVar v)  (act ?r'))\<longrightarrow> va \<in> (varOfFormList ?F)"
+      by auto  
+  qed
+
+lemma lemmaOnIdleGtNc:
+  assumes a1:"i>NC" and a2:"s \<in> reachableSet (set (allInitSpecs N)) (rules N)" and 
+a3:"NC<N" and  
+  a4:"\<forall>f.  f \<in>(set invariantsAbs) \<longrightarrow>  formEval f s"
+  shows "trans_sim_on1 (n_Idle  i) (n_ABS_Idle  NC) (set invariantsAbs) s" (is "trans_sim_on1 ?r ?r' ?F s")
+proof(rule ruleSimCond)
+  show " formEval (pre ?r) s \<longrightarrow>formEval (pre ?r') s" (is "?A \<longrightarrow>?B")
+  proof(rule impI)+
+    assume b1:"?A"  
+     have "(inv__5 0 1 )\<in>(set invariantsAbs)" by (force simp del:inv__5_def)
+     from a4  have b4:"formEval (inv__5 0 1 ) s" apply(force simp del:inv__5_def) done 
+
+    have b5:"formEval (inv__5 i 0 ) s" 
+    proof(cut_tac a1 a2 a3 b4,rule axiomOnf2,force+)qed
+    with b1  have b6:"formEval (neg (eqn (IVar (Field (Para (Ident ''n'') 0) ''st'')) (Const E))) s" by auto
+     have b7:"formEval (inv__5 i 1 ) s" 
+     proof(cut_tac a1 a2 a3 b4,rule axiomOnf2,force+)qed
+     with b1 have b7:"formEval (neg (eqn (IVar (Field (Para (Ident ''n'') 1) ''st'')) (Const E))) s" by auto
+
+     have "(inv__6 0 1 )\<in>(set invariantsAbs)" by force
+     with a4 have b8:"formEval (inv__6 0 1 ) s"  apply(drule_tac x="(inv__6 0 1 )" in spec,blast)done
+
+     have b9:"formEval (inv__6 i 0 ) s" 
+    proof(cut_tac a1 a2 a3 b8,rule axiomOnf2,force+)qed
+    with b1 have b9:"formEval (neg (eqn (IVar (Field (Para (Ident ''n'') 0) ''st'')) (Const C))) s" by auto
+     have b10:"formEval (inv__6 i 1 ) s" 
+     proof(cut_tac a1 a2 a3 b8,rule axiomOnf2,force+)qed
+     with b1 have b11:"formEval (neg (eqn (IVar (Field (Para (Ident ''n'') 1) ''st'')) (Const C))) s" by auto
+    
+     from b1 b6 b7 b9 b11 show "formEval (pre ?r') s" 
+       by auto
+   qed
+ next
+    
+   show "\<forall>v. v\<in>varOfForm (pre ?r') \<longrightarrow> v \<in>(varOfFormList invariantsAbs)"
+      by auto
+ next
+  
+   show "
+  (\<forall>v.   v \<in> (varOfFormList invariantsAbs) \<longrightarrow>formEval (pre ?r) s\<longrightarrow> expEval (substExpByStatement (IVar v)  (act ?r')) s = expEval (substExpByStatement (IVar v)  (act ?r)) s)"  
+   proof((rule allI)+,(rule impI)+,auto)
+     fix  v
+     assume b1:"v\<in> (varOfFormList invariantsAbs)"  and b2:"formEval (pre ?r) s"
+
+     have "(inv__3 0  )\<in>(set invariantsAbs)" by force
+     with a4 have b30:"formEval (inv__3 0 ) s"   apply(drule_tac x="(inv__3 0  )" in spec,blast)done
+
+     have b3:"formEval (inv__3 i ) s"  proof(cut_tac a1 a2 a3 b30,rule axiomOnf1,force+)qed
+
+     show "expEval (substExpByStatement (IVar v)  (act ?r')) s = expEval (substExpByStatement (IVar v)  (act ?r)) s"  
+       apply (cut_tac  a1 b1 b2 b3,auto) done
+   qed
+  (* have "\<forall>f v va. v \<in> varOfForm f \<longrightarrow> f \<in>?F \<longrightarrow>va\<in>varOfExp ( substExpByStatement (IVar v)  (act ?r'))\<longrightarrow> va \<in>(varOfFormList invariantsAbs)"   by auto*)
+     then show "\<forall> v va. v \<in> varOfFormList invariantsAbs \<longrightarrow>va\<in>varOfExp ( substExpByStatement (IVar v)  (act ?r'))\<longrightarrow> va \<in> varOfFormList invariantsAbs"
+      by auto  
+  qed
+
+
+
+lemma lemmaOnCritLeNc:
+  assumes a1:"i\<le>NC" 
+  shows "trans_sim_on1 (n_Crit  i) (n_Crit  i) (set invariantsAbs) s" (is "trans_sim_on1 ?r ?r ?F s")
+proof(rule ruleSimId)
+  show  "\<forall>v. v\<in>varOfForm (pre ?r) \<longrightarrow>  v \<in>(varOfFormList invariantsAbs) "
+    by(cut_tac a1, auto) 
+    
+next
+  show  b1: "\<forall>v a. a \<in> set (statement2Assigns (act ?r))
+ \<longrightarrow> v\<in>varOfExp ( substExpByStatement (IVar (fst a))  (act ?r))\<longrightarrow>v \<in>varOfFormList invariantsAbs "
+   proof((rule allI)+,(rule impI)+,auto) qed
+    
+qed
+
+lemma lemmaOnCritGtNc:
+  assumes a1:"i>NC" and a2:"s \<in> reachableSet (set (allInitSpecs N)) (rules N)" and a3:"NC<N" and  
+  a4:"\<forall>f.  f \<in>(set invariantsAbs) \<longrightarrow>  formEval f s"
+  shows "trans_sim_on1 (n_Crit  i) (n_ABS_Crit  ) (set invariantsAbs) s" (is "trans_sim_on1 ?r ?r' ?F s")
+proof(rule ruleSimCond)
+  show " formEval (pre ?r) s \<longrightarrow>formEval (pre ?r') s" (is "?A \<longrightarrow>?B")
+  proof(rule impI)+
+    assume b1:"?A"  
+     
+    
+     from b1  show "formEval (pre ?r') s" 
+       by auto
+   qed
+ next
+    
+   show "\<forall>v. v\<in>varOfForm (pre ?r') \<longrightarrow> v \<in>(varOfFormList invariantsAbs)"
+      by auto
+ next
+   
+   show "
+  (\<forall>v.   v \<in> (varOfFormList invariantsAbs) \<longrightarrow>formEval (pre ?r) s\<longrightarrow> expEval (substExpByStatement (IVar v)  (act ?r')) s = expEval (substExpByStatement (IVar v)  (act ?r)) s)"  
+   proof((rule allI)+,(rule impI)+)
+     fix  v
+     assume b1:"v\<in> (varOfFormList invariantsAbs)"  and b2:"formEval (pre ?r) s"
+    
+    
+
+     show "expEval (substExpByStatement (IVar v)  (act ?r')) s = expEval (substExpByStatement (IVar v)  (act ?r)) s"  
+       apply (cut_tac  a1 b1 b2 ,auto) done
+   qed
+  (* have "\<forall>f v va. v \<in> varOfForm f \<longrightarrow> f \<in>?F \<longrightarrow>va\<in>varOfExp ( substExpByStatement (IVar v)  (act ?r'))\<longrightarrow> va \<in>(varOfFormList invariantsAbs)"   by auto*)
+     then show "\<forall> v va. v \<in> varOfFormList invariantsAbs \<longrightarrow>va\<in>varOfExp ( substExpByStatement (IVar v)  (act ?r'))\<longrightarrow> va \<in> varOfFormList invariantsAbs"
+      by auto  
+  qed
+
+
+lemma lemmaOnStoreLeNc:
+  assumes a1:"i\<le>NC" 
+  shows "trans_sim_on1 (n_Store  i d) (n_Store  i d) (set invariantsAbs) s" (is "trans_sim_on1 ?r ?r ?F s")
+proof(rule ruleSimId)
+  show  "\<forall>v. v\<in>varOfForm (pre ?r) \<longrightarrow>  v \<in>(varOfFormList invariantsAbs) "
+    by(cut_tac a1, auto) 
+    
+next
+  show  b1: "\<forall>v a. a \<in> set (statement2Assigns (act ?r)) \<longrightarrow> v\<in>varOfExp ( substExpByStatement (IVar (fst a))  (act ?r))\<longrightarrow>v \<in>varOfFormList invariantsAbs "
+   proof(cut_tac a1,(rule allI)+,(rule impI)+,auto) qed
+    
+qed
+
+lemma lemmaOnStoreGtNc:
+  assumes a1:"i>NC" and a2:"s \<in> reachableSet (set (allInitSpecs N)) (rules N)" and a3:"1<N" and  
+  a4:"\<forall>f.  f \<in>(set invariantsAbs) \<longrightarrow>  formEval f s"
+  shows "trans_sim_on1 (n_Store  i d) (n_ABS_Store  NC d) (set invariantsAbs) s" (is "trans_sim_on1 ?r ?r' ?F s")
+proof(rule ruleSimCond)
+  show " formEval (pre ?r) s \<longrightarrow>formEval (pre ?r') s" (is "?A \<longrightarrow>?B")
+  proof(rule impI)+
+    assume b1:"?A"  
+     have "(inv__1 0 1 )\<in>(set invariantsAbs)" by force
+     with a4  have b4:"formEval (inv__1 0 1 ) s"  apply(drule_tac x="(inv__1 0 1 )" in spec,blast)done
+
+    have b5:"formEval (inv__1 i 0 ) s" 
+    proof(cut_tac a1 a2 a3 b4,rule axiomOnf2,force+)qed
+    with b1  have b6:"formEval (neg (eqn (IVar (Field (Para (Ident ''n'') 0) ''st'')) (Const C))) s" by auto
+     have b7:"formEval (inv__1 i 1 ) s" 
+     proof(cut_tac a1 a2 a3 b4,rule axiomOnf2,force+)qed
+     with b1 have b7:"formEval (neg (eqn (IVar (Field (Para (Ident ''n'') 1) ''st'')) (Const C))) s" by auto
+
+     have "(inv__4 0 1 )\<in>(set invariantsAbs)" by force
+     with a4 have b8:"formEval (inv__4 0 1 ) s"  apply(drule_tac x="(inv__4 0 1 )" in spec,blast)done
+
+     have b9:"formEval (inv__4 i 0 ) s" 
+    proof(cut_tac a1 a2 a3 b8,rule axiomOnf2,force+)qed
+    with b1 have b9:"formEval (neg (eqn (IVar (Field (Para (Ident ''n'') 0) ''st'')) (Const E))) s" by auto
+     have b10:"formEval (inv__4 i 1 ) s" 
+     proof(cut_tac a1 a2 a3 b8,rule axiomOnf2,force+)qed
+     with b1 have b11:"formEval (neg (eqn (IVar (Field (Para (Ident ''n'') 1) ''st'')) (Const E))) s" by auto
+    
+     from b1 b6 b7 b9 b11 show "formEval (pre ?r') s" 
+       by auto
+   qed
+ next
+    
+   show "\<forall>v. v\<in>varOfForm (pre ?r') \<longrightarrow> v \<in>(varOfFormList invariantsAbs)"
+      by auto
+ next
+   
+   show "
+  (\<forall>v.   v \<in> (varOfFormList invariantsAbs) \<longrightarrow>formEval (pre ?r) s\<longrightarrow> expEval (substExpByStatement (IVar v)  (act ?r')) s = expEval (substExpByStatement (IVar v)  (act ?r)) s)"  
+   proof((rule allI)+,(rule impI)+)
+     fix  v
+     assume b1:"v\<in> (varOfFormList invariantsAbs)"  and b2:"formEval (pre ?r) s"
+
+     have "(inv__3 0  )\<in>(set invariantsAbs)" by force
+     with a4 have b30:"formEval (inv__3 0 ) s"   apply(drule_tac x="(inv__3 0  )" in spec,blast)done
+
+     have b3:"formEval (inv__3 i ) s"  proof(cut_tac a1 a2 a3 b30,rule axiomOnf1,force+)qed
+
+     show "expEval (substExpByStatement (IVar v)  (act ?r')) s = expEval (substExpByStatement (IVar v)  (act ?r)) s"  
+       apply (cut_tac  a1 b1 b2 b3,auto) done
+   qed
+  (* have "\<forall>f v va. v \<in> varOfForm f \<longrightarrow> f \<in>?F \<longrightarrow>va\<in>varOfExp ( substExpByStatement (IVar v)  (act ?r'))\<longrightarrow> va \<in>(varOfFormList invariantsAbs)"   by auto*)
+     then show "\<forall> v va. v \<in> varOfFormList invariantsAbs \<longrightarrow>va\<in>varOfExp ( substExpByStatement (IVar v)  (act ?r'))\<longrightarrow> va \<in> varOfFormList invariantsAbs"
+      by auto  
+  qed
+
+lemma lemmaOnTryLeNc:
+  assumes a1:"i\<le>NC" 
+  shows (*"\<exists> r'. r' \<in> rulesAbs NC\<and> trans_sim_on1 (n_Try  i) r' (set invariantsAbs) s"*)
+ "trans_sim_on1 (n_Try  i) (n_Try  i) (set invariantsAbs) s" (is "trans_sim_on1 ?r ?r ?F s") 
+proof(rule ruleSimId)
+  show  "\<forall>v. v\<in>varOfForm (pre ?r) \<longrightarrow>  v \<in>(varOfFormList invariantsAbs) "
+    by(cut_tac a1, auto) 
+    
+next
+  show  b1: "\<forall>v a. a \<in> set (statement2Assigns (act ?r)) \<longrightarrow> 
+  v\<in>varOfExp ( substExpByStatement (IVar (fst a))  (act ?r))\<longrightarrow>v \<in>varOfFormList invariantsAbs "
+   proof(cut_tac a1,(rule allI)+,(rule impI)+,auto) qed
+    
+qed
+
+lemma lemmaOnTryGtNc:
+  assumes a1:"i>NC" and a2:"s \<in> reachableSet (set (allInitSpecs N)) (rules N)"  and  
+  a4:"\<forall>f.  f \<in>(set invariantsAbs) \<longrightarrow>  formEval f s"
+shows "trans_sim_on1 (n_Try  i) (n_Try  0) (set invariantsAbs) s" (is "trans_sim_on1 ?r ?r' ?F s")
+proof(unfold trans_sim_on1_def,(rule allI)+,(rule impI)+,rule disjI2)
+  fix s2 
+  assume b0:"state_sim_on1 s s2 (set invariantsAbs)"
+  show "state_sim_on1 (trans (act (n_Try i)) s) s2 (set invariantsAbs)"
+  proof(cut_tac a1,unfold state_sim_on1_def,
+    (rule allI)+,(rule impI)+)
+    fix f v
+    assume b1:" f \<in>(set invariantsAbs)" and b2:"v \<in> varOfForm f"  
+
+    have b30: "(varOfFormList  invariantsAbs) = {v. \<exists>f. f \<in> set  invariantsAbs\<and> v \<in> varOfForm f}"
+      using setOfList by blast
+      
+     
+    from b1 and b2 and b30 have b4:"v \<in> (varOfFormList  invariantsAbs)" by blast
+     
+    from b4 have b5:"trans (act (n_Try  i)) s v = s v" 
+      by (cut_tac a1  b4  ,auto) 
+
+    from b0   have b6:"s v =s2 v "
+      using b1 b2 state_sim_on1_def by blast  
+    show "trans (act (n_Try i)) s v= s2 v"
+      using b5 b6 by auto 
+  qed
+qed
+
+lemma lemmaOnTry: 
+  assumes   a2:"s \<in> reachableSet (set (allInitSpecs N)) (rules N)"  and  
+  a4:"\<forall>f.  f \<in>(set invariantsAbs) \<longrightarrow>  formEval f s" and a5:"\<exists>i. i\<le>N \<and> r=(n_Try  i)"
+  shows "\<exists> r'. r' \<in> rulesAbs NC\<and> trans_sim_on1 r r' (set invariantsAbs) s" (is "\<exists>r'.?P1 r' \<and> ?P2 r'")
+proof -
+  from a5 obtain i where d0:"i\<le>N \<and> r=(n_Try  i)"  by blast
+  have "i \<le> NC | i> NC" by auto
+  moreover{
+  assume a1:"i \<le>NC" 
+  have "\<exists>r'. ?P1 r' \<and> ?P2 r'"
+  proof(rule_tac x="(n_Try  i)" in exI,rule conjI)
+
+    show  "?P1 (n_Try  i) " 
+      by(cut_tac a1, auto) 
+    
+  next
+    show  "?P2 (n_Try  i) "
+      using lemmaOnTryLeNc local.a1 d0 by blast 
+  qed
+}
+ moreover{
+  assume a1:"i >NC" 
+  have "\<exists>r'. ?P1 r' \<and> ?P2 r'"
+  proof(rule_tac x="(n_Try  0)" in exI,rule conjI)
+
+    show  "?P1 (n_Try  0) " 
+      by(cut_tac a1, auto) 
+    
+  next
+    show  "?P2 (n_Try  0) "
+    
+      using lemmaOnTryGtNc local.a1 a2 a4 d0 by blast 
+  qed 
+}
+  ultimately show "\<exists>r'.?P1 r' \<and> ?P2 r'" 
+    by satx
+qed
+
+lemma lemmaOnExitLeNc:
+  assumes a1:"i\<le>NC" 
+  shows "trans_sim_on1 (n_Exit  i) (n_Exit  i) (set invariantsAbs) s" (is "trans_sim_on1 ?r ?r ?F s")
+proof(rule ruleSimId)
+  show  "\<forall>v. v\<in>varOfForm (pre ?r) \<longrightarrow>  v \<in>(varOfFormList invariantsAbs) "
+    by(cut_tac a1, auto) 
+    
+next
+  show  b1: "\<forall>v a. a \<in> set (statement2Assigns (act ?r)) \<longrightarrow> 
+  v\<in>varOfExp ( substExpByStatement (IVar (fst a))  (act ?r))\<longrightarrow>v \<in>varOfFormList invariantsAbs "
+   proof(cut_tac a1,(rule allI)+,(rule impI)+,auto) qed
+    
+qed
+
+lemma lemmaOnExitGtNc:
+  assumes a1:"i>NC" and a2:"s \<in> reachableSet (set (allInitSpecs N)) (rules N)" and a3:"NC<N" and  
+  a4:"\<forall>f.  f \<in>(set invariantsAbs) \<longrightarrow>  formEval f s"
+shows "trans_sim_on1 (n_Exit  i) (n_Exit  0) (set invariantsAbs) s" (is "trans_sim_on1 ?r ?r' ?F s")
+proof(unfold trans_sim_on1_def,(rule allI)+,(rule impI)+,rule disjI2)
+  fix s2 
+  assume b0:"state_sim_on1 s s2 (set invariantsAbs)"
+  show "state_sim_on1 (trans (act (n_Exit i)) s) s2 (set invariantsAbs)"
+  proof(cut_tac a1,unfold state_sim_on1_def,
+    (rule allI)+,(rule impI)+)
+    fix f v
+    assume b1:" f \<in>(set invariantsAbs)" and b2:"v \<in> varOfForm f"  
+
+    have b30: "(varOfFormList  invariantsAbs) = {v. \<exists>f. f \<in> set  invariantsAbs\<and> v \<in> varOfForm f}"
+      using setOfList by blast
+      
+     
+    from b1 and b2 and b30 have b4:"v \<in> (varOfFormList  invariantsAbs)" by blast
+     
+    from b4 have b5:"trans (act (n_Exit  i)) s v = s v" 
+      by (cut_tac a1  b4  ,auto) 
+
+    from b0   have b6:"s v =s2 v "
+      using b1 b2 state_sim_on1_def by blast  
+    show "trans (act (n_Exit i)) s v= s2 v"
+      using b5 b6 by auto 
+  qed
+qed
+
+lemma lemmaOnIdle: 
+  assumes   a2:"s \<in> reachableSet (set (allInitSpecs N)) (rules N)"  and  a1:"NC<N" and
+  a4:"\<forall>f.  f \<in>(set invariantsAbs) \<longrightarrow>  formEval f s" and a5:"\<exists>i. i\<le>N \<and> r=(n_Idle  i)"
+  shows "\<exists> r'. r' \<in> rulesAbs NC\<and> trans_sim_on1 r r' (set invariantsAbs) s" (is "\<exists>r'.?P1 r' \<and> ?P2 r'")
+proof -
+  from a5 obtain i where d0:"i\<le>N \<and> r=(n_Idle  i)"  by blast
+  have "i \<le> NC |  NC<i" by auto
+  moreover{
+  assume b1:"i \<le>NC" 
+  have "\<exists>r'. ?P1 r' \<and> ?P2 r'"
+  proof(rule_tac x="(n_Idle  i)" in exI,rule conjI)
+
+    show  "?P1 (n_Idle  i) " 
+      by(cut_tac b1, auto) 
+    
+  next
+    show  "?P2 (n_Idle  i) "
+      using lemmaOnIdleLeNc b1 d0 by blast 
+  qed
+}
+ moreover{
+  assume b1:"NC<i" 
+  have "\<exists>r'. ?P1 r' \<and> ?P2 r'"
+  proof(rule_tac x="(n_ABS_Idle  NC)" in exI,rule conjI)
+
+    show  "?P1 (n_ABS_Idle  NC) " 
+      by(cut_tac a1, auto) 
+    
+  next
+    show  "?P2 (n_ABS_Idle  NC) "  thm lemmaOnIdleGtNc
+   
+      using lemmaOnIdleGtNc b1 a1 a2 a4 d0 by blast 
+  qed 
+}
+  ultimately show "\<exists>r'.?P1 r' \<and> ?P2 r'" 
+    by satx
+qed
+
+lemma lemmaOnCrit: 
+  assumes   a2:"s \<in> reachableSet (set (allInitSpecs N)) (rules N)"  and  a1:"NC<N" and
+  a4:"\<forall>f.  f \<in>(set invariantsAbs) \<longrightarrow>  formEval f s" and a5:"\<exists>i. i\<le>N \<and> r=(n_Crit  i)"
+  shows "\<exists> r'. r' \<in> rulesAbs NC\<and> trans_sim_on1 r r' (set invariantsAbs) s" (is "\<exists>r'.?P1 r' \<and> ?P2 r'")
+proof -
+  from a5 obtain i where d0:"i\<le>N \<and> r=(n_Crit  i)"  by blast
+  have "i \<le> NC |  NC<i" by auto
+  moreover{
+  assume b1:"i \<le>NC" 
+  have "\<exists>r'. ?P1 r' \<and> ?P2 r'"
+  proof(rule_tac x="(n_Crit  i)" in exI,rule conjI)
+
+    show  "?P1 (n_Crit  i) " 
+      by(cut_tac b1, auto) 
+    
+  next
+    show  "?P2 (n_Crit  i) "
+      using lemmaOnCritLeNc b1 d0 by blast 
+  qed
+}
+ moreover{
+  assume b1:"NC<i" 
+  have "\<exists>r'. ?P1 r' \<and> ?P2 r'"
+  proof(rule_tac x="(n_ABS_Crit )" in exI,rule conjI)
+
+    show  "?P1 (n_ABS_Crit  ) " 
+      by(cut_tac a1, auto) 
+    
+  next
+    show  "?P2 (n_ABS_Crit ) "  thm lemmaOnIdleGtNc
+   
+      using lemmaOnCritGtNc b1 a1 a2 a4 d0 by blast 
+  qed 
+}
+  ultimately show "\<exists>r'.?P1 r' \<and> ?P2 r'" 
+    by satx
+qed
+
+
+lemma lemmaOnExit: 
+  assumes   a2:"s \<in> reachableSet (set (allInitSpecs N)) (rules N)"  and  a1:"NC<N" and
+  a4:"\<forall>f.  f \<in>(set invariantsAbs) \<longrightarrow>  formEval f s" and a5:"\<exists>i. i\<le>N \<and> r=(n_Exit  i)"
+  shows "\<exists> r'. r' \<in> rulesAbs NC\<and> trans_sim_on1 r r' (set invariantsAbs) s" (is "\<exists>r'.?P1 r' \<and> ?P2 r'")
+proof -
+  from a5 obtain i where d0:"i\<le>N \<and> r=(n_Exit  i)"  by blast
+  have "i \<le> NC |  NC<i" by auto
+  moreover{
+  assume b1:"i \<le>NC" 
+  have "\<exists>r'. ?P1 r' \<and> ?P2 r'"
+  proof(rule_tac x="(n_Exit  i)" in exI,rule conjI)
+
+    show  "?P1 (n_Exit  i) " 
+      by(cut_tac b1, auto) 
+    
+  next
+    show  "?P2 (n_Exit  i) "
+      using lemmaOnExitLeNc b1 d0 by blast 
+  qed
+} 
+moreover{
+  assume b1:"NC<i" 
+  have "\<exists>r'. ?P1 r' \<and> ?P2 r'"
+  proof(rule_tac x="(n_Exit  0)" in exI,rule conjI)
+
+    show  "?P1 (n_Exit  0) " 
+      by(cut_tac a1, auto) 
+    
+  next
+    show  "?P2 (n_Exit  0) "  thm lemmaOnExitGtNc
+    
+      using lemmaOnExitGtNc b1 a1 a2 a4 d0 by blast 
+  qed 
+}
+  ultimately show "\<exists>r'.?P1 r' \<and> ?P2 r'" 
+    by satx
+qed
+
+lemma simCond1: 
+  assumes a1:"s \<in>reachableSet (set (allInitSpecs N)) (rules N)" and
+    a2:"(\<forall> f. f \<in>(set invariantsAbs) \<longrightarrow> formEval f s )" and a3:"NC <N"
+
+  shows "prot_sim_on1 {andList (allInitSpecs N)} {andList (allInitSpecs NC)} 
+    (rules N) (rulesAbs NC) (set invariantsAbs) s" (is "prot_sim_on1 {?I} {?I'} ?rs ?rs' ?F s")
+proof(unfold prot_sim_on1_def,rule conjI)
+  show "\<forall>f. f \<in> {?I} \<longrightarrow> (\<exists>f'. f' \<in> {?I'} \<and> pred_sim_on1 f f' ?F s)"
+  proof(rule allI, rule impI)
+    fix i 
+    assume b1:" i \<in> {?I}"
+    show "(\<exists>f'. f' \<in> {?I'} \<and> pred_sim_on1 i f' ?F s)"
+    proof(rule_tac x="?I'" in exI,rule conjI)
+      show "pred_sim_on1 i ?I' ?F s"
+      proof(unfold pred_sim_on1_def,rule impI)
+        assume c1:"formEval i s"
+        show "(\<exists>s'. formEval ?I' s' \<and>  state_sim_on1 s s' ?F)"
+        proof(rule_tac x="s" in exI,cut_tac b1 c1 a3,rule conjI)
+          have "formEval (andList (allInitSpecs N)) s"
+            using b1 c1 by blast 
+          then show "formEval (andList (allInitSpecs NC)) s"
+          proof(cut_tac a3 ,auto simp del:evalEqn )
+          qed
+          
+          next
+            show " state_sim_on1 s s ?F"
+              by auto
+          qed
+        qed
+      next 
+        show "andList (allInitSpecs NC)  \<in> {andList (allInitSpecs NC)} " by blast
+      qed
+    
+    
+    qed
+  next 
+    show " (\<forall>r. r \<in> ?rs\<longrightarrow>(\<exists> r'. r' \<in> ?rs' \<and> trans_sim_on1 r r' (set invariantsAbs) s))" (is "?P")
+    proof(rule allI, rule impI)
+      fix r
+      assume b1:"r \<in> (rules N)"
+      have c1: "(\<exists> i. i\<le>N\<and>r=n_Try  i)\<or>
+      (\<exists> i. i\<le>N\<and>r=n_Crit  i)\<or>
+      (\<exists> i. i\<le>N\<and>r=n_Exit  i)\<or>
+      (\<exists> i. i\<le>N\<and>r=n_Idle  i)"
+          apply (cut_tac b1, auto) done
+    moreover {
+      assume d1: "(\<exists> i. i\<le>N\<and>r=n_Try  i)"
+          have "(\<exists> r'. r' \<in> ?rs' \<and> trans_sim_on1 r r' (set invariantsAbs) s)"
+            using a2 a1 d1 lemmaOnTry by blast 
+    }
+
+    moreover {
+      assume d1: "(\<exists> i. i\<le>N\<and>r=n_Exit  i)"
+          have "(\<exists> r'. r' \<in> ?rs' \<and> trans_sim_on1 r r' (set invariantsAbs) s)" thm lemmaOnExit
+            using a3 a2 a1 d1 lemmaOnExit by blast
+    }
+
+    moreover {
+      assume d1: "(\<exists> i. i\<le>N\<and>r=n_Idle  i)"
+          have "(\<exists> r'. r' \<in> ?rs' \<and> trans_sim_on1 r r' (set invariantsAbs) s)" thm lemmaOnExit
+            using a3 a2 a1 d1 lemmaOnIdle by blast
+    }
+
+
+  moreover {
+      assume d1: "(\<exists> i. i\<le>N\<and>r=n_Crit  i)"
+       have "(\<exists> r'. r' \<in> ?rs' \<and> trans_sim_on1 r r' (set invariantsAbs) s)" thm lemmaOnExit
+            using a3 a2 a1 d1 lemmaOnCrit  by blast
+    }
+
+  ultimately show "(\<exists> r'. r' \<in> ?rs' \<and> trans_sim_on1 r r' (set invariantsAbs) s)" 
+    by satx
+qed
+qed
+
+lemma iniImply_inv__1:
+assumes a1: "(\<exists> p__Inv3 p__Inv4. p__Inv3\<le>N\<and>p__Inv4\<le>N\<and>p__Inv3~=p__Inv4\<and>f=inv__1  p__Inv3 p__Inv4)"
+and a2: "formEval (andList (allInitSpecs N)) s"
+shows "formEval f s"
+  using a1 a2 apply( auto  )done
+
+lemma iniImply_inv__1:
+assumes a1: "(\<exists> p__Inv3 p__Inv4. p__Inv3\<le>NC\<and>p__Inv4\<le>NC\<and>p__Inv3~=p__Inv4\<and>f=inv__1  p__Inv3 p__Inv4)"
+and a2: "formEval (andList (allInitSpecs NC)) s"
+shows "formEval f s"
+using a1 a2 apply( auto  )done
+
+lemma iniImply_inv__2:
+assumes a1: "(\<exists> p__Inv4. p__Inv4\<le>N\<and>f=inv__2  p__Inv4)"
+and a2: "formEval (andList (allInitSpecs N)) s"
+shows "formEval f s"
+using a1 a2 by (auto )
+
+lemma iniImply_inv__3:
+assumes a1: "(\<exists> p__Inv3 p__Inv4. p__Inv3\<le>N\<and>p__Inv4\<le>N\<and>p__Inv3~=p__Inv4\<and>f=inv__3  p__Inv3 p__Inv4)"
+and a2: "formEval (andList (allInitSpecs N)) s"
+shows "formEval f s"
+using a1 a2 by auto
+
+lemma iniImply_inv__4:
+assumes a1: "(\<exists> p__Inv4. p__Inv4\<le>N\<and>f=inv__4  p__Inv4)"
+and a2: "formEval (andList (allInitSpecs N)) s"
+shows "formEval f s"
+using a1 a2 by auto
+
+lemma iniImply_inv__5:
+assumes a1: "(\<exists> p__Inv3 p__Inv4. p__Inv3\<le>N\<and>p__Inv4\<le>N\<and>p__Inv3~=p__Inv4\<and>f=inv__5  p__Inv3 p__Inv4)"
+and a2: "formEval (andList (allInitSpecs N)) s"
+shows "formEval f s"
+using a1 a2 by auto
+
+end
+      show "(\<exists> r'. r' \<in> ?rs' \<and> trans_sim_on1 r r' (set invariantsAbs) s)"
+      
+  qed
+end          
+set fs \<subseteq>  invs ; ( \<forall> inv. inv \<in>invs \<longrightarrow>formEval inv s
+(\<forall>f. f \<in> I \<longrightarrow> (\<exists>f'. f' \<in> I' \<and> pred_sim_on1 f f' F s)) \<and>
+  (\<forall>r. r \<in> rs\<longrightarrow>(\<exists> r'. r' \<in> rs' \<and> trans_sim_on1 r r' F s))
+assumes  a1:"\<forall>s. s \<in>reachableSet I rs \<longrightarrow> (\<forall> f. f \<in>F \<longrightarrow> formEval f s )\<longrightarrow>prot_sim_on1 I I' rs rs' F s"
+    and a2:"\<forall>s f. s \<in>reachableSet I' rs' \<longrightarrow>f \<in>F \<longrightarrow> formEval f s  "
+  (*and a3:"\<forall>s. s \<in>reachableSet I rs' \<longrightarrow>f \<in>F \<longrightarrow> formEval f s  " *)
+  and a4:"s \<in>reachableSet I rs " and a5:"\<forall> s f.  f \<in>I \<longrightarrow> formEval f s \<longrightarrow> (\<forall>f'. f' \<in>F \<longrightarrow> formEval  f' s)   "
+  and a6:"\<forall> s f.  f \<in>I' \<longrightarrow> formEval f s \<longrightarrow> (\<forall>f'. f' \<in>F \<longrightarrow> formEval  f' s)   "
+lemma lemmaOnTryGtNc:
+  assumes a1:"i>NC" and a2:"s \<in> reachableSet (set (allInitSpecs N)) (rules N)" and a3:"1<N"
+  shows "trans_sim_on1 (n_Idle  i) (n_ABS_Idle  NC) (set invariantsAbs) s" (is "trans_sim_on1 ?r ?r' ?F s")
+proof(rule ruleSimCond)
+  show " (\<forall> f. f \<in>?F \<longrightarrow> formEval f s ) \<longrightarrow> formEval (pre ?r) s \<longrightarrow>formEval (pre ?r') s" (is "?A \<longrightarrow>?B\<longrightarrow>?C")
+  proof(rule impI)+
+    assume b1:"?A" and b2:"?B" 
+    from b1 have b4:"formEval (inv__5 0 1 ) s"  by auto
+    have b5:"formEval (inv__5 i 0 ) s" 
+    proof(cut_tac a1 a2 a3 b4,rule axiomOnf2,force+)qed
+    with b2 have b6:"formEval (neg (eqn (IVar (Field (Para (Ident ''n'') 0) ''st'')) (Const E))) s" by auto
+     have b7:"formEval (inv__5 i 1 ) s" 
+     proof(cut_tac a1 a2 a3 b4,rule axiomOnf2,force+)qed
+     with b2 have b7:"formEval (neg (eqn (IVar (Field (Para (Ident ''n'') 1) ''st'')) (Const E))) s" by auto
+
+     from b1 have b8:"formEval (inv__6 0 1 ) s"  by auto
+     have b9:"formEval (inv__6 i 0 ) s" 
+    proof(cut_tac a1 a2 a3 b8,rule axiomOnf2,force+)qed
+    with b2 have b9:"formEval (neg (eqn (IVar (Field (Para (Ident ''n'') 0) ''st'')) (Const C))) s" by auto
+     have b10:"formEval (inv__6 i 1 ) s" 
+     proof(cut_tac a1 a2 a3 b8,rule axiomOnf2,force+)qed
+     with b2 have b11:"formEval (neg (eqn (IVar (Field (Para (Ident ''n'') 1) ''st'')) (Const C))) s" by auto
+    
+     from b2 b6 b7 b9 b11 show "formEval (pre ?r') s" 
+       by auto
+   qed
+ next
+   have "\<forall>v. v\<in>varOfForm (pre ?r') \<longrightarrow> v \<in>(varOfFormList invariantsAbs)"
+     by simp
+   then show "\<forall>v. v\<in>varOfForm (pre ?r') \<longrightarrow>(\<exists>f. f \<in>?F \<and>v \<in> varOfForm f)"
+     using mem_Collect_eq setOfList by auto
+ next
+   
+   show " (\<forall> f. f \<in>?F \<longrightarrow> formEval f s ) \<longrightarrow>
+  (\<forall>f  v. f\<in> ?F \<longrightarrow>  v \<in> varOfForm f \<longrightarrow>formEval (pre ?r) s\<longrightarrow> expEval (substExpByStatement (IVar v)  (act ?r')) s = expEval (substExpByStatement (IVar v)  (act ?r)) s)" (is "?A \<longrightarrow>?B")
+   proof(rule impI)+
+     assume b1:"?A" 
+    
+     from b1 have b2:"formEval (inv__3 0 ) s"   by auto
+
+     have b2:"formEval (inv__3 i ) s"  proof(cut_tac a1 a2 a3 b2,rule axiomOnf1,force+)qed
+     show "?B"  by (cut_tac a1 b2,auto)
+   qed
+   have "\<forall>f v va. v \<in> varOfForm f \<longrightarrow> f \<in>?F \<longrightarrow>va\<in>varOfExp ( substExpByStatement (IVar v)  (act ?r'))\<longrightarrow> va \<in>(varOfFormList invariantsAbs)"   by auto
+     then show "\<forall>f v va. v \<in> varOfForm f \<longrightarrow> f \<in>?F \<longrightarrow>va\<in>varOfExp ( substExpByStatement (IVar v)  (act ?r'))\<longrightarrow> (\<exists>f. f \<in>?F \<and>va \<in> varOfForm f)"
+     using mem_Collect_eq setOfList by auto  
+ qed
+
+end
+and
+  a5:"\<forall>f v va. v \<in> varOfForm f \<longrightarrow> f \<in>F \<longrightarrow>va\<in>varOfExp ( substExpByStatement (IVar v)  (act r2))\<longrightarrow> (varOfFormList invariantsAbs)"  
+*)
